theories/interop/wrapper_wp_ext_call_laws.v
@@ -240,6 +240,154 @@ Proof.
       - intros ℓ γ [HH1 HH2]%lookup_delete_Some; by eapply Hrootslive.
 Qed.
 
+Lemma list_insert_lookup_inv  A (vs:list A) (i:nat) v k : k ∈ <[ i := v ]> vs → k = v ∨ k ∈ vs.
+Proof.
+  induction vs as [|vh vs IH] in i|-*.
+  - intros []%elem_of_nil.
+  - destruct i; cbn.
+    + intros [<- | Hvs]%elem_of_cons; first by left. by do 2 right.
+    + intros [<- | Hvs]%elem_of_cons; first (right; by left).
+      destruct (IH _ Hvs) as [-> | Hr]; first by left.
+      by do 2 right.
+Qed.
+
+Lemma wp_ext_call_modify : ext_call_is_sound WP_modify_spec.
+Proof.
+  intros E T s vv K Ξ Φ.
+  rewrite weakestpre.wp_unfold. rewrite /weakestpre.wp_pre.
+  iIntros "%Hnone Hnb HT IH %σ Hσ".
+  destruct σ as [ρml σ | ρc mem].
+  1: iExFalso; iNamed "Hσ"; iNamed "SIML"; iPoseProof (ghost_var_agree with "Hnb HAbound") as "%HH"; congruence.
+  iNamed "Hσ"; iNamed "SIC".
+  cbn. unfold WP_modify_spec. iNamed "HT". iNamed "HGC".
+  iPoseProof (ghost_var_agree with "HAGCθ HAθ") as "%H"; subst θ.
+  iPoseProof (lstore_own_mut_of with "HAζrest Hpto") as "%Helem". destruct Helem as [Helem _].
+  iAssert ⌜ζC ρc !! γ = Some (Mut, (tg, vs))⌝%I as "%Helem2".
+  1: { iPureIntro. eapply lookup_union_Some_r in Helem; last apply Hfreezedj.
+       rewrite <- Hfreezeeq in Helem.
+       destruct Hfreezeρ as [HL HR].
+       assert (γ ∈ dom (ζC ρc)) as [v Hv]%elem_of_dom by by (rewrite HL; eapply elem_of_dom_2).
+       specialize (HR _ _ _ Hv Helem) as Hinv. inversion Hinv; subst; done. }
+
+  iModIntro. iRight. iRight. iSplitR.
+  + iPureIntro. econstructor. eapply head_prim_step.
+    eapply (PrimModifyS _ _ _ _ _ _ _ _ _ _ _ _ _ (fun k => True)); try done.
+    eapply mk_modify_block. lia.
+  + iIntros (X Hstep).
+    destruct Hstep as ([] & x & Hre & Hstep). change (fill () x) with x in Hre. subst x.
+    cbn in Hstep; unfold step,mrel in Hstep; cbn in Hstep.
+    inversion_call_step Hstep ([ w; #i; w' ]). subst.
+    iMod (lstore_own_update _ _ _ _ blk' with "HAζrest Hpto") as "(HAζrest&Hpto)".
+    iPoseProof (sigma_None_extract with "HAσMLv HAχNone") as "%Hpublocs".
+
+    do 3 iModIntro.
+    do 2 iExists _. change (Wrap.fill () ?x) with (x) in H10.
+    inversion Hreprw; inversion H4; subst; injection H14; intros ->.
+    destruct HGCOK as [HGCL HGCR]. assert (γ = γ0) as <- by by eapply HGCL.
+    assert (lv = v') as -> by by eapply repr_lval_inj_1.
+    iSplitR; first (iPureIntro; eapply H10).
+    iSplitR "Hnb IH HWP HAGCθ HAGCbound HArootss HArootsm Hrootspto Hpto".
+    * cbn. unfold C_state_interp. iSplitL "HσC HnC"; first (iExists nCv; iFrame).
+      iExists (<[γ:=blk']> (ζσ ∪ ζrest)), ζσ, (<[γ:=blk']>ζrest), χvirt, σMLvirt.
+      inversion H7; subst.
+      iFrame. iSplitL "HAnMLv"; first by iExists _.
+      erewrite pub_locs_in_lstore_insert_existing; last by eapply elem_of_dom_2.
+      iFrame; iPureIntro; split_and!; try done. 1: destruct Hfreezeρ as [HL HR]; split.
+      - erewrite !dom_insert_L, HL. done.
+      - intros γ' b1 b2 [[? ?]|[Hne1 H1]]%lookup_insert_Some [[??]|[Hne2 H2']]%lookup_insert_Some; try congruence.
+        1: subst; econstructor.
+        subst. by eapply HR.
+      - rewrite insert_union_r; first done.
+        erewrite map_disjoint_Some_l; done.
+      - eapply map_disjoint_dom. erewrite dom_insert_lookup; last by eexists. by eapply map_disjoint_dom.
+      - rewrite dom_insert_lookup; last by eexists. 
+        done.
+      - intros ℓ Vs γ1 bb H1 H2' [[<- <-]|[Hne H3']]%lookup_insert_Some.
+        -- epose proof (map_Forall_lookup_1 _ _ γ ℓ Hpublocs) as Hpub2. cbn in Hpub2.
+           rewrite Hpub2 in H1; first congruence.
+           eapply pub_locs_in_lstore_lookup; last apply H2'.
+           eapply elem_of_dom_2; done.
+        -- specialize (Hstore _ _ _ _ H1 H2' H3'); inversion Hstore; subst.
+           econstructor. eapply Forall2_impl; first done.
+           intros x y HH; eapply is_val_insert_immut; last done.
+           1: erewrite lookup_union_r; first done.
+           1: eapply map_disjoint_Some_l; done. done.
+      - split; first apply HGCL.
+        intros γ0 m1 tg1 vs1 γ1 Hγ0 [[??]|[Hne1 Hlu]]%lookup_insert_Some Hlloc.
+        2: by eapply HGCR.
+        injection H9; intros <- <- <-. subst γ0.
+        rewrite Helem2 in H5; injection H5; intros <- <-.
+        apply list_insert_lookup_inv in Hlloc as [HLL|HRR].
+        2: { eapply HGCR; try done.
+             erewrite lookup_union_r; first done.
+             1: eapply map_disjoint_Some_l; done. }
+        subst v'. inversion H6; subst. by eapply elem_of_dom_2.
+    * iApply ("IH" with "[-Hnb] Hnb").
+      inversion H7; subst.
+      rewrite Helem2 in H5; injection H5; intros <- <-. change (Z.of_nat 0) with (Z0).
+      iApply ("HWP" with "[-Hpto] [Hpto]").
+      2: iSplitL; done.
+      iExists _, _. iFrame. done.
+Qed.
+
+Lemma wp_ext_call_readfield : ext_call_is_sound WP_readfield_spec.
+Proof.
+  intros E T s vv K Ξ Φ.
+  rewrite weakestpre.wp_unfold. rewrite /weakestpre.wp_pre.
+  iIntros "%Hnone Hnb HT IH %σ Hσ".
+  destruct σ as [ρml σ | ρc mem].
+  1: iExFalso; iNamed "Hσ"; iNamed "SIML"; iPoseProof (ghost_var_agree with "Hnb HAbound") as "%HH"; congruence.
+  iNamed "Hσ"; iNamed "SIC".
+  cbn. unfold WP_readfield_spec. iNamed "HT". iNamed "HGC".
+  iPoseProof (ghost_var_agree with "HAGCθ HAθ") as "%H"; subst θ.
+  iPoseProof (lstore_own_elem_of with "HAζrest Hpto") as "%Helem".
+  iAssert ⌜∃ m', ζC ρc !! γ = Some (m', (tg, vs))⌝%I as "%Helem2".
+  1: { iPureIntro. eapply lookup_union_Some_r in Helem; last apply Hfreezedj.
+       rewrite <- Hfreezeeq in Helem.
+       destruct Hfreezeρ as [HL HR].
+       assert (γ ∈ dom (ζC ρc)) as [v Hv]%elem_of_dom by by (rewrite HL; eapply elem_of_dom_2).
+       specialize (HR _ _ _ Hv Helem) as Hinv. inversion Hinv; subst; by eexists. }
+  destruct Helem2 as [m' Helem2].
+  assert (exists (vv:lval), vs !! (Z.to_nat i) = Some vv) as [vv Hvv].
+  1: apply lookup_lt_is_Some; lia.
+  destruct HGCOK as [HGCL HGCR].
+  inversion Hreprw; subst.
+
+  assert (exists w', repr_lval (θC ρc) vv w') as [w' Hw'].
+  1: { destruct vv as [vvz|vvl]; first (eexists; econstructor).
+       eapply elem_of_dom in HGCR as [w' Hw']; first (eexists; by econstructor).
+       1: eapply elem_of_dom_2, H1.
+       2: by eapply elem_of_list_lookup_2.
+       erewrite lookup_union_r; first done.
+       eapply map_disjoint_Some_l; done. }
+
+  iModIntro. iRight. iRight. iSplitR.
+  + iPureIntro. econstructor. eapply head_prim_step.
+    eapply (PrimReadfieldS _ _ _ _ _ _ _ _ _ _ _ _ _ (fun k => True)); done.
+  + iIntros (X Hstep).
+    destruct Hstep as ([] & x & Hre & Hstep). change (fill () x) with x in Hre. subst x.
+    cbn in Hstep; unfold step,mrel in Hstep; cbn in Hstep.
+    inversion_call_step Hstep ([ #a ; #i ]). subst.
+
+    inversion H5; subst. assert (γ = γ0) as <- by by eapply HGCL.
+    rewrite Helem2 in H6; injection H6; intros <- <- <-.
+    rewrite Hvv in H7; injection H7; intros <-.
+    assert (w'0 = w') as -> by by eapply repr_lval_inj.
+
+    do 3 iModIntro.
+    do 2 iExists _. change (Wrap.fill () ?x) with (x) in H10.
+    iSplitR; first (iPureIntro; eapply H10).
+
+    iSplitR "Hnb IH HWP HAGCθ HAGCbound HArootss HArootsm Hrootspto Hpto".
+    * cbn. unfold C_state_interp. iSplitL "HσC HnC"; first (iExists nCv; iFrame).
+      iExists ((ζσ ∪ ζrest)), ζσ, (ζrest), χvirt, σMLvirt.
+      iFrame. iSplitL "HAnMLv"; first by iExists _.
+      done.
+    * iApply ("IH" with "[-Hnb] Hnb").
+      iApply ("HWP" with "[-Hpto] [Hpto] [] []"); try done.
+      iExists _, _; iFrame; done.
+Qed.
+
 Ltac solve_ext_call H := 
     iPoseProof (H with "[] Hnb H [IH]") as "Hwp"; [done
     | iIntros "!> %r HΞ Hnb"; iApply ("IH" with "HΞ Hnb"); by iApply "Hr"
@@ -258,11 +406,14 @@ Proof.
   destruct σ as [ρml σ | ρc mem].
   1: iExFalso; iNamed "Hσ"; iNamed "SIML"; iPoseProof (ghost_var_agree with "Hnb HAbound") as "%HH"; congruence.
   iNamed "Hσ"; iNamed "SIC".
-  cbn. iDestruct "HT" as "[H|[H|[H|H]]]".
+  cbn. iDestruct "HT" as "[H|[H|[H|[H|[H|H]]]]]".
   - solve_ext_call wp_ext_call_int2val.
   - solve_ext_call wp_ext_call_val2int.
   - solve_ext_call wp_ext_call_registerroot.
   - solve_ext_call wp_ext_call_unregisterroot.
+  - solve_ext_call wp_ext_call_modify.
+  - solve_ext_call wp_ext_call_readfield.
+  (* - solve_ext_call wp_ext_call_alloc. *)
 Qed.
 
 
